\documentclass{article}
\usepackage{ifthen}
\usepackage{epsfig}
\usepackage[utf8]{inputenc}
% Packages requested by user
\usepackage{amsmath}

\usepackage{newunicodechar}
  \newunicodechar{⁻}{${}^{-}$}% Superscript minus
  \newunicodechar{²}{${}^{2}$}% Superscript two
  \newunicodechar{³}{${}^{3}$}% Superscript three

\pagestyle{empty}
\begin{document}
$p$
\pagebreak

$q$
\pagebreak

$\theta$
\pagebreak

$\phi$
\pagebreak

$x$
\pagebreak

$y$
\pagebreak

$P$
\pagebreak

$Q$
\pagebreak

$\theta = 0$
\pagebreak

$\theta = \pi/2$
\pagebreak

$\phi = 0$
\pagebreak

$\tilde{\theta}$
\pagebreak

\[ \tilde{\theta} = \frac{\pi}{2} - \theta. \]
\pagebreak

${\bf P}$
\pagebreak

$(a,b)$
\pagebreak

$(c,d)$
\pagebreak

\[ {\bf P}_{(a,b)\rightarrow(c,d)} \equiv \begin{bmatrix} P_{ca} & P_{cb} \\ P_{da} & P_{db} \end{bmatrix} \equiv \begin{bmatrix} \frac{\partial c}{\partial a} & \frac{\partial c}{\partial b} \\[5 pt] \frac{\partial d}{\partial a} & \frac{\partial d}{\partial b} \end{bmatrix} \]
\pagebreak

$\chi$
\pagebreak

$(x,y)\rightarrow(\theta,\phi)$
\pagebreak

$\pi - \chi$
\pagebreak

\[ {\bf P}_\text{pa} = \begin{bmatrix} P_{\theta x} & P_{\theta y} \\ P_{\phi x} & P_{\phi y} \end{bmatrix} = \begin{bmatrix} \cos\left(\pi - \chi\right) & -\sin\left(\pi - \chi\right) \\ \sin\left(\pi - \chi\right) & \cos\left(\pi - \chi\right) \end{bmatrix} = \begin{bmatrix} -\cos\chi & -\sin\chi \\ \sin\chi & -\cos\chi \end{bmatrix}. \]
\pagebreak

\[ \tan \chi = \frac{\cos \lambda \sin H}{\sin\lambda \cos x - \cos \lambda \sin x \cos H}, \]
\pagebreak

$\lambda$
\pagebreak

$H$
\pagebreak

$\lambda_\text{MWA} = -0.4660608448386394$
\pagebreak

$N_t$
\pagebreak

$N_f$
\pagebreak

$N_a$
\pagebreak

$N_p$
\pagebreak

${\bf D}$
\pagebreak

\[ N_a \times N_f \times N_p \times N_p, \]
\pagebreak

$D_{a,f,p_1,p_2}$
\pagebreak

\[ {\bf e} = \begin{bmatrix} e_x \\ e_y \end{bmatrix}, \]
\pagebreak

\[ {\bf J} = \begin{bmatrix} J_{xx} & J_{xy} \\ J_{yx} & J_{yy} \end{bmatrix}. \]
\pagebreak

$i$
\pagebreak

$N_i = N_a \times N_p$
\pagebreak

$\{I, Q, U, V\}$
\pagebreak

$N_s$
\pagebreak

$N_d = 16$
\pagebreak

$N_b$
\pagebreak

$N_d$
\pagebreak

${\bf J}$
\pagebreak

${\bf B}$
\pagebreak

${\bf G}$
\pagebreak

${\bf E}$
\pagebreak

$2\times2$
\pagebreak

${\bf e}$
\pagebreak

${\bf v}$
\pagebreak

\[ {\bf v} = {\bf J}{\bf e}. \]
\pagebreak

\[ \begin{bmatrix} v_q \\ v_p \end{bmatrix} = \begin{bmatrix} J_{qx} & J_{qy} \\ J_{px} & J_{py} \end{bmatrix} \begin{bmatrix} e_x \\ e_y \end{bmatrix}, \]
\pagebreak

\[ {\bf e} = {\bf J}^{-1}{\bf v}. \]
\pagebreak

\[ {\bf J} = {\bf D}{\bf B}, \]
\pagebreak

${\bf J}_d$
\pagebreak

${\bf B}_\text{cal}$
\pagebreak

${\bf J}_b$
\pagebreak

\begin{align*} {\bf J}_d &= \begin{bmatrix} J_{px} & J_{py} \\ J_{qx} & J_{qy} \end{bmatrix}, & {\bf J}_b &= \begin{bmatrix} J_{px} & J_{py} \\ J_{qx} & J_{qy} \end{bmatrix}, & {\bf B}_\text{cal} &= \begin{bmatrix} B_{px} & B_{py} \\ B_{qx} & B_{qy} \end{bmatrix}. \end{align*}
\pagebreak

\[ {\bf J} = {\bf J}_d \]
\pagebreak

\[ {\bf J} = {\bf J}_d {\bf J}_b \]
\pagebreak

\[ {\bf D} = {\bf J}{\bf B}_\text{cal}^{-1}. \]
\pagebreak

\[ {\bf D} = \begin{bmatrix} D_{pp} & D_{pq} \\ D_{qp} & D_{qq} \end{bmatrix}. \]
\pagebreak

\[ {\bf D} = \begin{bmatrix} D_{qq} & D_{qp} \\ D_{pq} & D_{pp} \end{bmatrix}. \]
\pagebreak

\[ {\bf B}_\text{hb} = \begin{bmatrix} B_{q\theta} & B_{q\phi} \\ B_{p\theta} & B_{p\phi} \end{bmatrix}. \]
\pagebreak

$(x,y)$
\pagebreak

$(q,p)$
\pagebreak

${\bf B}_\text{hb}$
\pagebreak

\[ {\bf B} = {\bf B}_\text{hb}{\bf P}_\text{pa} = \begin{bmatrix} B_{q\theta} & B_{q\phi} \\ B_{p\theta} & B_{p\phi} \end{bmatrix} \begin{bmatrix} P_{\theta x} & B_{\theta y} \\ B_{\phi x} & B_{\phi y} \end{bmatrix} = \begin{bmatrix} B_{qx} & B_{qy} \\ B_{px} & B_{py} \end{bmatrix} \]
\pagebreak

\[ {\bf e}_f = \frac{1}{N_a} \sum_a e^{i\varphi_{a,f}} {\bf J}_{a,f}^{-1} {\bf v}_{a,f}, \]
\pagebreak

$a$
\pagebreak

$f$
\pagebreak

$\varphi$
\pagebreak

${\bf J}_{a,f}^{-1}$
\pagebreak

${\bf v}_{a,f}$
\pagebreak

$e^{i\varphi_{a,f}})$
\pagebreak

${\bf D}_a$
\pagebreak

${\bf B}_{a,f}$
\pagebreak

\[ {\bf J}_{a,f} = {\bf D}_a {\bf B}_{a,f} \]
\pagebreak

${\bf B}_f$
\pagebreak

${\bf J}^{-1}$
\pagebreak

\[ \tilde{\bf e}_{a,f} = {\bf J}^{-1}_{a,f} {\bf v}_{a,f}. \]
\pagebreak

$e^{i\varphi}$
\pagebreak

\[ {\bf e}_{a,f} = e^{i\varphi_f} \tilde{\bf e}_{a,f}. \]
\pagebreak

\[ {\bf e}_f = \frac{1}{N_a}\sum_a \tilde{\bf e}_{a,f}. \]
\pagebreak

\[ {\bf e}{\bf e}^\dagger = \begin{bmatrix} e_x e_x^\ast & e_x e_y^\ast \\ e_y e_x^\ast & e_y e_y^\ast \end{bmatrix} = \frac12 \begin{bmatrix} I + Q & U + Vi \\ U - Vi & I - Q \end{bmatrix} \]
\pagebreak

\[ \frac12 \begin{bmatrix} I + Q & U + Vi \\ U - Vi & I - Q \end{bmatrix} = {\bf e}{\bf e}^\dagger - \sum_a {\bf e}_a {\bf e}_a^\dagger. \]
\pagebreak

$D$
\pagebreak

$(Q,P)$
\pagebreak

\[\begin{bmatrix} D_{qq} & D_{qp} \\ D_{pq} & D_{pp} \end{bmatrix}.\]
\pagebreak

$(P,Q)$
\pagebreak

\[ \begin{bmatrix} D_{pp} & D_{pq} \\ D_{qp} & D_{qq} \end{bmatrix} \rightarrow \begin{bmatrix} D_{qq} & D_{qp} \\ D_{pq} & D_{pp} \end{bmatrix} \]
\pagebreak

${\bf J}_m$
\pagebreak

${\bf J}_f$
\pagebreak

${\bf J}_\text{ref}$
\pagebreak

\[ \begin{aligned} {\bf J} &= \begin{bmatrix} J_0 & J_1 \\ J_2 & J_3 \end{bmatrix}, & {\bf J}_\text{ref} &= \begin{bmatrix} J_{\text{ref},0} & J_{\text{ref},1} \\ J_{\text{ref},2} & J_{\text{ref},3} \end{bmatrix}, \end{aligned} \]
\pagebreak

\[ \begin{bmatrix} J_0\frac{|J_{\text{ref},0}|}{J_{\text{ref},0}} & J_1\frac{|J_{\text{ref},1}|}{J_{\text{ref},1}} \\ J_2\frac{|J_{\text{ref},2}|}{J_{\text{ref},2}} & J_3\frac{|J_{\text{ref},3}|}{J_{\text{ref},3}}. \end{bmatrix} \]
\pagebreak

\[ {\bf J} = \begin{bmatrix} J_0 & J_1 \\ J_2 & J_3 \end{bmatrix} \rightarrow \begin{bmatrix} J_0 & 0 \\ 0 & J_3 \end{bmatrix}. \]
\pagebreak

$z$
\pagebreak

$z^N = 1$
\pagebreak

$v$
\pagebreak

$N_t \times N_f \times N_i$
\pagebreak

$I$
\pagebreak

$N_t \times N_f$
\pagebreak

\[ I_{t,f} = \sum_i v_{t,f,i}^\dagger v_{t,f,i}. \]
\pagebreak

$\langle\langle\langle(N_f, N_t), N_i\rangle\rangle\rangle.$
\pagebreak

\[ I_{t,f} = \sum_a {\bf v}_{t,f,a}^\dagger {\bf v}_{t,f,a}. \]
\pagebreak

$N_a \times N_f \times N_p \times N_p$
\pagebreak

${\bf J}^{-1}{\bf v}$
\pagebreak

$N_t \times N_f \times N_a$
\pagebreak

\[ \tilde{\bf e}_{t,f,a} = {\bf J}^{-1}_{a,f}{\bf v}_{t,f,a}. \]
\pagebreak

$\langle\langle\langle(N_f, N_t), N_a\rangle\rangle\rangle.$
\pagebreak

$N_a \times N_f$
\pagebreak

$N_t \times N_f \times N_p$
\pagebreak

$N_t \times N_s \times N_f$
\pagebreak

\[ {\bf e}_{t,f} = \frac{1}{N_a} \sum_a e^{i\varphi} \tilde{\bf e}_{t,f,a}. \]
\pagebreak

$S = [I, Q, U, V]$
\pagebreak

${\bf S}$
\pagebreak

\[ \hat{\bf S} = \frac{{\bf S} - \text{offset}}{\text{scale}}, \]
\pagebreak

\begin{align*} \text{scale} &= \frac{S_\text{max} - S_\text{min}}{256} \\ \text{offset} &= S_\text{min} + 0.5 \times \text{scale}. \end{align*}
\pagebreak

$\langle\langle\langle N_b,(N_f, N_s)\rangle\rangle\rangle.$
\pagebreak

${\bf J}^{-1} {\bf v}$
\pagebreak

${\bf J}^{-1} = \left({\bf D}{\bf B}\right)^{-1}$
\pagebreak

\[ \begin{aligned} {\bf e} &= {\bf J}^{-1} {\bf v}, \\ \begin{bmatrix} e_x \\ e_y \end{bmatrix} &= \begin{bmatrix} J_{xq} & J_{xp} \\ J_{yq} & J_{yp} \end{bmatrix} \begin{bmatrix} v_q \\ v_p \end{bmatrix}. \end{aligned} \]
\pagebreak

\[{\bf J}^{-1} = \left({\bf D}{\bf B}\right)^{-1},\]
\pagebreak

$(N_a \times N_f \times N_p \times N_p)$
\pagebreak

${\bf M}_\text{in}$
\pagebreak

${\bf M}_\text{out} = {\bf M}_\text{in}$
\pagebreak

$\dfrac{1}{z}$
\pagebreak

$-z$
\pagebreak

${\bf M}_\text{out} = {\bf M}_\text{in}^{-1}$
\pagebreak

${\bf M}_1$
\pagebreak

${\bf M}_2$
\pagebreak

${\bf M}_\text{out} = {\bf M}_1 \times {\bf M}_2$
\pagebreak

${\bf M}$
\pagebreak

${\bf M}_\text{out} = {\bf M}^\ast$
\pagebreak

${\bf M}_\text{out} = |{\bf M}_\text{in}|$
\pagebreak

${\bf M}_\text{out}$
\pagebreak

\[\begin{bmatrix} 0 & 1 \\ 2 & 3\end{bmatrix} \rightarrow \begin{bmatrix} 3 & 2 \\ 1 & 0 \end{bmatrix}\]
\pagebreak

\[\begin{bmatrix} 0 & 1 \\ 2 & 3\end{bmatrix} \rightarrow \begin{bmatrix} 2 & 3 \\ 0 & 1 \end{bmatrix}\]
\pagebreak

\[\begin{bmatrix} 0 & 1 \\ 2 & 3\end{bmatrix} \rightarrow \begin{bmatrix} 1 & 0 \\ 3 & 2 \end{bmatrix}\]
\pagebreak

${\bf H} = {\bf M}^\dagger$
\pagebreak

${\bf C} = {\bf M}{\bf M}^\dagger$
\pagebreak

${\bf J}{\bf v}$
\pagebreak

\[ X_k[m] \sum_n^{K-1} b_m[n] e^{-2\pi jkn/K}, \]
\pagebreak

\[ b_m[n] = \sum_\rho^{P-1} h[K\rho - n] x[n + mM - K\rho]. \]
\pagebreak

$X$
\pagebreak

$h$
\pagebreak

$b$
\pagebreak

$\text{nspectra}$
\pagebreak

$K$
\pagebreak

$x[n]$
\pagebreak

$h[n]$
\pagebreak

$b[n]$
\pagebreak

$ \langle\langle\langle (\text{nspectra},I,P), K \rangle\rangle\rangle $
\pagebreak

\[ \begin{cases} \left\lfloor \frac{x}{2^{14}} + 0.5 \right\rfloor, & x > 0, \\ \left\lfloor \frac{x}{2^{14}} \right\rfloor, & x \le 0. \end{cases} \]
\pagebreak

$\langle\langle\langle (\text{nspectra} \times I), K \rangle\rangle\rangle$
\pagebreak

$\langle\langle\langle(\text{nspectra},K),I\rangle\rangle\rangle$
\pagebreak

$M = K$
\pagebreak

\[ \hat{x}[n] = \frac{1}{K} \sum_m f[n - mM] \sum_{k=0}^{K-1} X_k[m]\,e^{2\pi jkn/K} \]
\pagebreak

$X_k[m]$
\pagebreak

$f[n]\,e^{2\pi jkn/K}$
\pagebreak

$N = KP$
\pagebreak

$\hat{x}[n]$
\pagebreak

\[ \text{result}[i] = f[n] \times exp{2\pi jk/K}, \]
\pagebreak

$n = i \% N$
\pagebreak

$k = i / N$
\pagebreak

$N$
\pagebreak

\[ {\bf B} = \begin{bmatrix} B_{qx} & B_{qy} \\ B_{px} & B_{py} \end{bmatrix}. \]
\pagebreak

$N_b \times N_a \times N_p \times N_p$
\pagebreak

$N_i \times N_d$
\pagebreak

$N_i$
\pagebreak

${\bf P}_\text{pa}$
\pagebreak

\[ {\bf P}_\text{pa} = \begin{bmatrix} P_{\theta x} & P_{\theta y} \\ P_{\phi x} & P_{\phi y} \end{bmatrix}. \]
\pagebreak

\end{document}
